Setlec/SetR.lean
@@ -146,6 +146,7 @@ import Setlec.SetR.Interp2.IndMemberP
 import Setlec.SetR.Interp2.IndCapsP
 import Setlec.SetR.Interp2.IndMembersP
 import Setlec.SetR.Interp2.IndTeleP
+import Setlec.SetR.Interp2.IndUnitLawP
 import Setlec.SetR.Interp2.AxiomPinP
 import Setlec.SetR.Interp2.HarvestP
 import Setlec.SetR.Interp2.FoldP
